Code cleanup
No functional changes.  Removed unneeded fields and renamed various
things, to improve readability.

libs/ml/FFICallbacks.ml
@@ -1,7 +1,7 @@
-type cookie = int
-external ocaml_send_tcp2: cookie -> string -> int = "ocaml_send_tcp"
-external ocaml_recv_tcp2: cookie -> string -> int = "ocaml_recv_tcp"
+type callbacks = int
+external ocaml_send_tcp2: callbacks -> string -> int = "ocaml_send_tcp"
+external ocaml_recv_tcp2: callbacks -> string -> int = "ocaml_recv_tcp"
 
-let ocaml_send_tcp cookie b = ocaml_send_tcp2 cookie b
-let ocaml_recv_tcp cookie b = ocaml_recv_tcp2 cookie b
+let ocaml_send_tcp callbacks b = ocaml_send_tcp2 callbacks b
+let ocaml_recv_tcp callbacks b = ocaml_recv_tcp2 callbacks b
 
