libs/ml/FFICallbacks.mli
@@ -1,4 +1,4 @@
-type cookie = int
-val ocaml_send_tcp: cookie -> string -> int
-val ocaml_recv_tcp: cookie -> string -> int
+type callbacks = int
+val ocaml_send_tcp: callbacks -> string -> int
+val ocaml_recv_tcp: callbacks -> string -> int
 
